refactor grw_mon expr to allow for gallina rewriting

src/grw_mon.v
@@ -3,19 +3,17 @@ Require CrossCrypto.fmap.
 Require Import FCF.FCF FCF.EqDec.
 Require Import Coq.Classes.Morphisms.
 Require Import CrossCrypto.RewriteUtil.
+Require Import Coq.derive.Derive.
+Require Import Coq.Logic.Eqdep_dec.
 
-Definition mapops V := list_of_pairs (V:=V) (Nat.eqb).
-Notation map V := (mapops V).(fmap.M).
-Notation mempty := (mapops _).(fmap.empty).
-Notation madd := (mapops _).(fmap.add).
-Notation mfind := (mapops _).(fmap.find).
-Notation mfold := (mapops _).(fmap.fold_ac).
-
-Inductive type : Type :=
+Inductive type : Set :=
 | tunit : type
 | tnat : type
 | tbool : type
 | tprod : type -> type -> type.
+
+Lemma type_dec (t1 t2 : type) : {t1 = t2} + {t1 <> t2}.
+Proof. decide equality. Defined.
 
 Bind Scope etype_scope with type.
 Delimit Scope etype_scope with etype.
@@ -39,6 +37,14 @@ Definition cfunc (t1 t2 : type) : Type :=
 Definition func (t1 t2 : type) : Type :=
   interp_type t1 -> Comp (interp_type t2).
 
+Definition ccompose {t1 t2 t3} (f : cfunc t1 t2) (g : cfunc t2 t3)
+  : cfunc t1 t3 :=
+  fun x => g (f x).
+
+Definition ctensor {t1 t2 t1' t2'} (f : cfunc t1 t2) (f' : cfunc t1' t2')
+  : cfunc (tprod t1 t1') (tprod t2 t2') :=
+  fun '(x, x') => (f x, f' x').
+
 Definition liftc {t1 t2 : type} (cf : cfunc t1 t2) : func t1 t2 :=
   fun x => ret (cf x).
 
@@ -50,17 +56,330 @@ Definition ftensor {t1 t2 t1' t2'} (f : func t1 t2) (f' : func t1' t2')
   : func (tprod t1 t1') (tprod t2 t2') :=
   fun '(x, x') => y <-$ f x; y' <-$ f' x'; ret (y, y').
 
+Inductive box_const : type -> type -> Type :=
+| bxor : box_const (tbool * tbool) tbool
+| bzero : box_const tunit tbool.
+
+Definition box_const_sigT_dec {t1 t2 t1' t2'}
+           (b : box_const t1 t2) (b' : box_const t1' t2') :
+  let P := fun '(t1, t2) => box_const t1 t2 : Type in
+  {existT P (t1, t2) b = existT P (t1', t2') b'} +
+  {existT P (t1, t2) b <> existT P (t1', t2') b'}.
+  intros; destruct b; destruct b';
+    solve [left; eauto |
+           right; intro; inversion_sigma; congruence].
+Defined.
+
+Definition box_const_dec {t1 t2} (b b' : box_const t1 t2)
+  : {b = b'} + {b <> b'}.
+  destruct (box_const_sigT_dec b b').
+  - left.
+    apply inj_pair2_eq_dec with (P := fun '(t1, t2) => box_const t1 t2 : Type)
+                                (p := (t1, t2)); eauto.
+    decide equality; eauto using type_dec.
+  - right; congruence.
+Defined.
+
+Inductive box : type -> type -> Type :=
+| bconst {t1 t2} : box_const t1 t2 -> box t1 t2
+| id {t} : box t t
+| assoc {t1 t2 t3} : box ((t1 * t2) * t3) (t1 * (t2 * t3))
+| iassoc {t1 t2 t3} : box (t1 * (t2 * t3)) ((t1 * t2) * t3)
+| unit_l {t} : box (tunit * t) t
+| iunit_l {t} : box t (tunit * t)
+| unit_r {t} : box (t * tunit) t
+| iunit_r {t} : box t (t * tunit)
+| copy {t} : box t (t * t)
+| delete {t} : box t tunit
+| swap {t1 t2} : box (t1 * t2) (t2 * t1)
+| bcompose {t1 t2 t3} : box t1 t2 -> box t2 t3 -> box t1 t3
+| btensor {t1 t1' t2 t2'} :
+    box t1 t2 -> box t1' t2' -> box (t1 * t1') (t2 * t2').
+
+Bind Scope box_scope with box.
+Delimit Scope box_scope with box.
+
+Local Notation "'#' x" := (bconst x)
+                            (no associativity,
+                             at level 9,
+                             format "# x") : box_scope.
+Local Notation "f1 * f2" := (btensor f1%box f2%box)
+                              (left associativity,
+                               at level 40) : box_scope.
+Local Notation "f @ g" := (bcompose f%box g%box)
+                            (right associativity,
+                             at level 41) : box_scope.
+
+Fixpoint size (t : type) : nat :=
+  match t with
+  | tprod t1 t2 => S (size t1 + size t2)
+  | _ => 1
+  end.
+
+Lemma bconst_eq_inv {t1 t2 : type} (b b' : box_const t1 t2) :
+  bconst b = bconst b' ->
+  existT (fun '(t1, t2) => box_const t1 t2 : Type)
+         (t1, t2) b =
+  existT (fun '(t1, t2) => box_const t1 t2 : Type)
+         (t1, t2) b'.
+Proof.
+  intros.
+  set (f (e : box t1 t2) :=
+         match e with
+         | @bconst t1 t2 b => existT _ (t1, t2) b
+         | _ => existT (fun '(t1, t2) => box_const t1 t2) (t1, t2) b
+         end).
+  change (f (bconst b) = f (bconst b')).
+  f_equal; eauto.
+Defined.
+
+Lemma bcompose_eq_inv {t1 t2 t2' t3 : type}
+      (b1 : box t1 t2) (b2 : box t2 t3)
+      (b1' : box t1 t2') (b2' : box t2' t3)  :
+  bcompose b1 b2 = bcompose b1' b2' ->
+  existT (fun '(t1, t2) => box t1 t2 : Type)
+         (t1, t2) b1 =
+  existT (fun '(t1, t2) => box t1 t2 : Type)
+         (t1, t2') b1' /\
+  existT (fun '(t1, t2) => box t1 t2 : Type)
+         (t2, t3) b2 =
+  existT (fun '(t1, t2) => box t1 t2 : Type)
+         (t2', t3) b2'.
+Proof.
+  intros.
+  set (f (e : box t1 t3) :=
+         match e with
+         | @bcompose t1 t2 t3 b1 b2 => existT _ (t1, t2) b1
+         | _ => existT (fun '(t1, t2) => box t1 t2) (t1, t2) b1
+         end).
+  set (g (e : box t1 t3) :=
+         match e with
+         | @bcompose t1 t2 t3 b1 b2 => existT _ (t2, t3) b2
+         | _ => existT (fun '(t1, t2) => box t1 t2) (t2, t3) b2
+         end).
+  split.
+  - change (f (bcompose b1 b2) = f (bcompose b1' b2')).
+    f_equal; eauto.
+  - change (g (bcompose b1 b2) = g (bcompose b1' b2')).
+    f_equal; eauto.
+Defined.
+
+Lemma btensor_eq_inv {t1 t1' t2 t2' : type}
+      (b1 b1' : box t1 t2) (b2 b2' : box t1' t2') :
+  btensor b1 b2 = btensor b1' b2' ->
+  existT (fun '(t1, t2) => box t1 t2 : Type)
+         (t1, t2) b1 =
+  existT (fun '(t1, t2) => box t1 t2 : Type)
+         (t1, t2) b1' /\
+  existT (fun '(t1, t2) => box t1 t2 : Type)
+         (t1', t2') b2 =
+  existT (fun '(t1, t2) => box t1 t2 : Type)
+         (t1', t2') b2'.
+Proof.
+  intros.
+  set (f (e : box (t1 * t1') (t2 * t2')) :=
+         match e with
+         | @btensor t1 t1' t2 t2' b1 b2 => existT _ (t1, t2) b1
+         | _ => existT (fun '(t1, t2) => box t1 t2) (t1, t2) b1
+         end).
+  set (g (e : box (t1 * t1') (t2 * t2')) :=
+         match e with
+         | @btensor t1 t1' t2 t2' b1 b2 => existT _ (t1', t2') b2
+         | _ => existT (fun '(t1, t2) => box t1 t2) (t1', t2') b2
+         end).
+  split.
+  - change (f (btensor b1 b2) = f (btensor b1' b2')).
+    f_equal; eauto.
+  - change (g (btensor b1 b2) = g (btensor b1' b2')).
+    f_equal; eauto.
+Defined.
+
+Ltac disprove_recursion :=
+  multimatch goal with
+  | H : ?a = _ |- _ =>
+    apply (f_equal size) in H;
+    cbn [size] in H;
+    omega
+  end.
+
+Ltac type_head x :=
+  match x with
+  | tunit => idtac
+  | tnat => idtac
+  | tbool => idtac
+  | tprod _ _ => idtac
+  end.
+
+Definition box_sigT_dec {t1 t2 t1' t2'} (b : box t1 t2)
+           (b' : box t1' t2') :
+  let P := fun '(t1, t2) => box t1 t2 : Type in
+  {existT P (t1, t2) b = existT P (t1', t2') b'} +
+  {existT P (t1, t2) b <> existT P (t1', t2') b'}.
+  intros.
+
+  revert t1' t2' b'.
+  induction b; intros ? ? b'; destruct b';
+    try solve [right;
+               intro;
+               inversion_sigma;
+               match goal with
+               | H : (_, _) = (_, _) |- _ => inversion H
+               end;
+               repeat match goal with
+                      | H : ?x = ?y |- _ => type_head x;
+                                            type_head y;
+                                            inversion H;
+                                            clear H
+                      end;
+               try disprove_recursion;
+               subst;
+               rewrite <- eq_rect_eq_dec in * by
+                   (decide equality; eauto using type_dec);
+               congruence];
+    match goal with
+    | |- {existT _ (?t1, ?t2) _ =
+          existT _ (?t1', ?t2') _} + {_} =>
+      destruct (type_dec t1 t1') as [e1|?];
+        [|right; intro; inversion_sigma; congruence];
+        inversion e1; subst;
+          solve [eauto] ||
+                (destruct (type_dec t2 t2') as [e2|?];
+                 [|right; intro; inversion_sigma; congruence];
+                 inversion e2; subst; eauto)
+    end.
+  - destruct (box_const_dec b b0). (* TODO name *)
+    + subst; eauto.
+    + right.
+      intro.
+      inversion_sigma.
+      match goal with
+      | H : (_, _) = (_, _) |- _ => inversion H
+      end.
+      subst.
+      rewrite <- eq_rect_eq_dec in * by
+          (decide equality; eauto using type_dec).
+      match goal with
+      | H : bconst _ = bconst _ |- _ => apply bconst_eq_inv in H
+      end.
+      inversion_sigma.
+      rewrite <- eq_rect_eq_dec in * by
+          (decide equality; eauto using type_dec).
+      congruence.
+  - destruct (IHb1 _ _ b'1). (* TODO name *)
+    + destruct (IHb2 _ _ b'2). (* TODO name *)
+      * inversion_sigma.
+        match goal with
+        | H : (_, _) = (_, _) |- _ => inversion H
+        end.
+        subst.
+        repeat rewrite <- eq_rect_eq_dec in * by
+            (decide equality; eauto using type_dec).
+        eauto.
+      * right.
+        intro.
+        inversion_sigma.
+        match goal with
+        | H : (_, _) = (_, _) |- _ => inversion H
+        end.
+        rewrite <- eq_rect_eq_dec in * by
+            (decide equality; eauto using type_dec).
+        match goal with
+        | H : bcompose _ _ = bcompose _ _ |- _ => apply bcompose_eq_inv in H;
+                                                    destruct H
+        end.
+        inversion_sigma.
+        subst.
+        rewrite <- eq_rect_eq_dec in * by
+            (decide equality; eauto using type_dec).
+        congruence.
+    + right.
+      intro.
+      inversion_sigma.
+      match goal with
+      | H : (_, _) = (_, _) |- _ => inversion H
+      end.
+      rewrite <- eq_rect_eq_dec in * by
+          (decide equality; eauto using type_dec).
+      match goal with
+      | H : bcompose _ _ = bcompose _ _ |- _ => apply bcompose_eq_inv in H;
+                                                  destruct H
+      end.
+      inversion_sigma.
+      inversion H4. (* TODO naming *)
+      subst.
+      rewrite <- eq_rect_eq_dec in * by
+          (decide equality; eauto using type_dec).
+      congruence.
+  - destruct (IHb1 _ _ b'1). (* TODO name *)
+    + destruct (IHb2 _ _ b'2). (* TODO name *)
+      * inversion_sigma.
+        match goal with
+        | H : (_, _) = (_, _) |- _ => inversion H
+        end.
+        subst.
+        repeat rewrite <- eq_rect_eq_dec in * by
+            (decide equality; eauto using type_dec).
+        eauto.
+      * right.
+        intro.
+        inversion_sigma.
+        match goal with
+        | H : (_, _) = (_, _) |- _ => inversion H
+        end.
+        rewrite <- eq_rect_eq_dec in * by
+            (decide equality; eauto using type_dec).
+        match goal with
+        | H : btensor _ _ = btensor _ _ |- _ => apply btensor_eq_inv in H;
+                                                  destruct H
+        end.
+        inversion_sigma.
+        subst.
+        rewrite <- eq_rect_eq_dec in * by
+            (decide equality; eauto using type_dec).
+        congruence.
+    + right.
+      intro.
+      inversion_sigma.
+      match goal with
+      | H : (_, _) = (_, _) |- _ => inversion H
+      end.
+      rewrite <- eq_rect_eq_dec in * by
+          (decide equality; eauto using type_dec).
+      match goal with
+      | H : btensor _ _ = btensor _ _ |- _ => apply btensor_eq_inv in H;
+                                                destruct H
+      end.
+      inversion_sigma.
+      subst.
+      rewrite <- eq_rect_eq_dec in * by
+          (decide equality; eauto using type_dec).
+      congruence.
+Defined.
+
+Lemma box_dec t1 t2 (b1 b2 : box t1 t2) : {b1 = b2} + {b1 <> b2}.
+Proof.
+  destruct (box_sigT_dec b1 b2).
+  - inversion_sigma.
+    subst.
+    rewrite <- eq_rect_eq_dec in * by
+        (decide equality; eauto using type_dec).
+    eauto.
+  - right; congruence.
+Defined.
+
+Inductive fconst : type -> type -> Type :=
+| coin : fconst tunit tbool.
+
 Inductive expr : type -> type -> Type :=
-| cconst {t1 t2} : cfunc t1 t2 -> expr t1 t2
-| const {t1 t2} : func t1 t2 -> expr t1 t2
+| ebox {t1 t2} : box t1 t2 -> expr t1 t2
+| const {t1 t2} : fconst t1 t2 -> expr t1 t2
 | compose {t1 t2 t3} : expr t1 t2 -> expr t2 t3 -> expr t1 t3
 | tensor {t1 t1' t2 t2'} :
     expr t1 t2 -> expr t1' t2' -> expr (tprod t1 t1') (tprod t2 t2').
 
 Bind Scope expr_scope with expr.
 Delimit Scope expr_scope with expr.
-Local Notation "'[[' x ']]'" := (cconst x)
-                            (format "[[ x ]]") : expr_scope.
+Local Notation "[[ x ]]" := (ebox x%box) : expr_scope.
 Local Notation "'#' x" := (const x)
                             (no associativity,
                              at level 9,
@@ -72,109 +391,243 @@ Local Notation "f @ g" := (compose f%expr g%expr)
                             (right associativity,
                              at level 41) : expr_scope.
 
+Definition interp_box_const {t1 t2} (c : box_const t1 t2) : cfunc t1 t2 :=
+  match c with
+  | bxor => fun '(x, y) => xorb x y
+  | bzero => fun _ => false
+  end.
+
+Fixpoint interp_box {t1 t2} (b : box t1 t2) : cfunc t1 t2 :=
+  match b with
+  | bconst c => interp_box_const c
+  | id => fun x => x
+  | assoc => fun '((x, y), z) => (x, (y, z))
+  | iassoc => fun '(x, (y, z)) => ((x, y), z)
+  | unit_l => fun '(_, x) => x
+  | iunit_l => fun x => (tt, x)
+  | unit_r => fun '(x, _) => x
+  | iunit_r => fun x => (x, tt)
+  | copy => fun x => (x, x)
+  | delete => fun _ => tt
+  | swap => fun '(x, y) => (y, x)
+  | bcompose b1 b2 => ccompose (interp_box b1) (interp_box b2)
+  | btensor b1 b2 => ctensor (interp_box b1) (interp_box b2)
+  end.
+
+Definition interp_fconst {t1 t2} (f : fconst t1 t2) : func t1 t2 :=
+  match f with
+  | coin => fun _ => x <-$ Rnd 1; ret (Vector.nth x Fin.F1)
+  end.
+
 Fixpoint interp_expr {t1 t2} (e : expr t1 t2) : func t1 t2 :=
   match e with
-  | [[cf]] => liftc cf
-  | #f => f
+  | [[b]] => liftc (interp_box b)
+  | #f => (interp_fconst f)
   | e1 @ e2 => fcompose (interp_expr e1) (interp_expr e2)
   | e * e' => ftensor (interp_expr e) (interp_expr e')
   end%expr.
 
-Fixpoint tmap (m : map type) : type :=
+Fixpoint tlist (m : list type) : type :=
   match m with
   | nil => tunit
-  | cons (_, t) m => tprod t (tmap m)
+  | cons t m => t * (tlist m)
   end.
 
-(* empty is just id_unit *)
+Fixpoint type_inhabited {t : type} : interp_type t :=
+  match t with
+  | tunit => tt
+  | tbool => false
+  | tnat => 0%nat
+  | tprod t1 t2 => (type_inhabited, type_inhabited)
+  end.
 
-Definition find (m : map type) (i : nat) (l : interp_type (tmap m))
-  : match mfind i m with
-    | Some t => interp_type t
-    | None => unit
-    end.
-  cbv [fmap.find mapops list_of_pairs].
-  induction m as [|[n t] m]; cbn [interp_type tmap find option_map] in l |- *.
-  - exact tt.
-  - destruct (n =? i); cbn [option_map snd].
-    + exact (fst l).
-    + apply IHm; exact (snd l).
+(* empty is just @id unit *)
+
+Fixpoint tindex (m : list type) (i : nat) {struct i} : type :=
+  match i with
+  | 0 => match m with
+         | nil => tunit
+         | cons t _ => t
+         end
+  | S i => match m with
+           | nil => tunit
+           | cons _ m => tindex m i
+           end
+  end.
+
+Definition ffst {t1 t2} : box (t1 * t2) t1 := (id * delete) @ unit_r.
+Definition fsnd {t1 t2} : box (t1 * t2) t2 := (delete * id) @ unit_l.
+
+Definition index (m : list type) (i : nat) :
+  box (tlist m) (tindex m i).
+  revert m.
+  induction i as [|i]; intros m.
+  - destruct m; cbn [tindex interp_type tlist] in *.
+    + exact delete.
+    + exact ffst.
+  - destruct m; cbn [tindex interp_type tlist] in *.
+    + exact delete.
+    + eapply bcompose.
+      * exact fsnd.
+      * eapply IHi.
 Defined.
 
-Definition add (m : map type) (i : nat) (t : type) (x : interp_type t)
-  (l : interp_type (tmap m)) : interp_type (tmap (madd i t m)) := (x, l).
-
-Definition fadd {m : map type} (i : nat) {t : type}
-  : cfunc (tprod t (tmap m)) (tmap (madd i t m)) :=
-  fun '(x, l) => add m i t x l.
-
-Definition copy {t} : cfunc t (tprod t t) :=
-  fun x => (x, x).
-Definition delete {t} : cfunc t tunit :=
-  fun _ => tt.
-Definition swap {t1 t2} : cfunc (tprod t1 t2) (tprod t2 t1) :=
-  fun '(t1, t2) => (t2, t1).
+(* add is id *)
 
 Definition units (t : type) :
-  cfunc tunit
-        ((fix units_type t :=
-            match t with
-            | t1 * t2 =>
-              (units_type t1) * (units_type t2)
-            | _ => tunit
-            end%etype) t).
+  box tunit
+      ((fix units_type t :=
+          match t with
+          | t1 * t2 =>
+            (units_type t1) * (units_type t2)
+          | _ => tunit
+          end%etype) t).
   induction t; try exact delete.
-  intros ?; cbn [interp_type]; eauto.
+  eapply bcompose.
+  - exact copy.
+  - eapply btensor; eauto.
 Defined.
 
-Definition fequiv {t1 t2} (f f' : func t1 t2) : Prop :=
-  forall x, Comp_eq (f x) (f' x).
+Definition fequiv {t1 t2} : func t1 t2 -> func t1 t2 -> Prop :=
+  pointwise_relation _ Comp_eq.
 
 Local Instance Equivalence_fequiv {t1 t2} : Equivalence (@fequiv t1 t2).
-Proof.
-  split; cbv [fequiv Reflexive Symmetric Transitive]; intros;
-    solve [(reflexivity + symmetry + etransitivity); eauto].
-Qed.
+Proof. typeclasses eauto. Qed.
 
-Definition cfequiv {t1 t2} (f f' : cfunc t1 t2) : Prop :=
-  forall x, f x = f' x.
+Definition cfequiv {t1 t2} : cfunc t1 t2 -> cfunc t1 t2 -> Prop :=
+  pointwise_relation _ eq.
 
 Local Instance Equivalence_cfequiv {t1 t2} : Equivalence (@cfequiv t1 t2).
-Proof.
-  split; cbv [cfequiv Reflexive Symmetric Transitive]; intros;
-    solve [(reflexivity + symmetry + etransitivity); eauto].
-Qed.
+Proof. typeclasses eauto. Qed.
 
-Lemma cfequiv_fequiv {t1 t2} (f f' : cfunc t1 t2) :
-  cfequiv f f' -> fequiv (liftc f) (liftc f').
+Local Existing Instance eq_subrelation | 5.
+
+Local Instance Proper_liftc {t1 t2} :
+  Proper (cfequiv ==> fequiv) (@liftc t1 t2).
 Proof.
-  cbv [cfequiv fequiv liftc].
-  intros H ?; setoid_rewrite H; reflexivity.
+  intros ????.
+  cbv [liftc].
+  setoid_rewrite H.
+  reflexivity.
 Qed.
 
 Definition equiv {t1 t2} (e e' : expr t1 t2) : Prop :=
   fequiv (interp_expr e) (interp_expr e').
 
 Local Instance Equivalence_equiv {t1 t2} : Equivalence (@equiv t1 t2).
+Proof. typeclasses eauto. Qed.
+
+Local Instance Proper_interp_expr {t1 t2} :
+  Proper (equiv ==> fequiv) (@interp_expr t1 t2).
+Proof. intros ???; eauto. Qed.
+
+Local Instance Proper_equiv_compose {t1 t2 t3} :
+  Proper (equiv ==> equiv ==> equiv) (@compose t1 t2 t3).
 Proof.
-  split; cbv [equiv Reflexive Symmetric Transitive]; intros;
-    solve [(reflexivity + symmetry + etransitivity); eauto].
+  cbv [equiv fequiv pointwise_relation].
+  intros ???????.
+  cbn [interp_expr].
+  cbv [fcompose].
+  f_equiv; eauto.
 Qed.
 
+Local Instance Proper_equiv_tensor {t1 t2 t3 t4} :
+  Proper (equiv ==> equiv ==> equiv) (@tensor t1 t2 t3 t4).
+Proof.
+  cbv [equiv fequiv pointwise_relation].
+  intros f f' Hf g g' Hg [].
+  cbn [interp_expr].
+  cbv [ftensor].
+  setoid_rewrite Hf.
+  setoid_rewrite Hg.
+  reflexivity.
+Qed.
+
+Lemma compose_assoc {t1 t2 t3 t4}
+      (f : expr t1 t2) (g : expr t2 t3) (h : expr t3 t4) :
+  equiv ((f @ g) @ h) (f @ (g @ h)).
+Proof.
+  cbv [equiv fequiv].
+  cbn [interp_expr].
+  cbv [fcompose].
+  setoid_rewrite <-Bind_assoc.
+  reflexivity.
+Qed.
+
+Lemma interchange {s1 s2 s3 t1 t2 t3}
+      (f1 : expr s1 s2) (f2 : expr s2 s3)
+      (g1 : expr t1 t2) (g2 : expr t2 t3) :
+  equiv ((f1 * g1) @ (f2 * g2)) ((f1 @ f2) * (g1 @ g2)).
+Proof.
+  cbv [equiv fequiv].
+  cbn [interp_expr].
+  cbv [fcompose ftensor].
+  intros [].
+  repeat setoid_rewrite <-Bind_assoc.
+  setoid_rewrite Bind_Ret_l.
+  f_equiv; intros ?.
+  setoid_rewrite Bind_comm with
+      (c1 := interp_expr f2 _) (c2 := interp_expr g1 _).
+  reflexivity.
+Qed.
+
+Lemma id_l {t1 t2} (x : expr t1 t2) : equiv ([[id]] @ x) x.
+Admitted.
+Lemma delete_r {t1 t2} (x : expr t1 t2) : equiv (x @ [[delete]]) [[delete]].
+Admitted.
+
+Lemma index_0_add {t m} :
+  equiv [[index (cons t m) 0]] [[ffst]].
+Proof. reflexivity. Qed.
+
+Lemma index_S_add {t m} n :
+  equiv [[index (cons t m) (S n)]] ([[fsnd]] @ [[index m n]]).
+Proof.
+  intro.
+  cbn [interp_expr].
+  cbv [liftc fcompose].
+  setoid_rewrite Bind_Ret_l.
+  reflexivity.
+Qed.
+
+Fixpoint associate_type (t : type) : type :=
+  match t with
+  | tprod t1 t2 =>
+    match associate_type t1 with
+    | tunit => associate_type t2
+    | t1' => match associate_type t2 with
+             | tunit => t1'
+             | tprod t2a t2b => tprod (tprod t1' t2a) t2b
+             | t2' => tprod t1' t2'
+             end
+    end
+  | _ => t
+  end.
+
+Fixpoint associate (t : type) : box t (associate_type t).
+  induction t; cbn [associate_type]; try exact id.
+  refine ((IHt1 * IHt2) @ _)%box.
+  destruct (associate_type t1); try exact unit_l;
+    destruct (associate_type t2);
+    exact id || exact unit_r || exact iassoc.
+Defined.
+
+Definition unassociate (t : type) : box (associate_type t) t.
+  induction t; cbn [associate_type interp_type]; try exact id.
+  refine (_ @ (IHt1 * IHt2))%box.
+  destruct (associate_type t1); try exact iunit_l;
+    destruct (associate_type t2);
+    exact id || exact iunit_r || exact assoc.
+Defined.
+
 Section ExampleCoins.
-  Definition coin : func tunit tbool :=
-    fun _ => x <-$ Rnd 1; ret (Vector.nth x Fin.F1).
-
-  Definition xor' : cfunc (tprod tbool tbool) tbool :=
-    fun '(x, y) => xorb x y.
-
   Lemma coins_xor :
     equiv ([[units (tunit * tunit)]]
              @ (#coin * #coin)
-             @ [[xor']])
+             @ [[#bxor]])
           #coin.
   Proof.
-    cbv [equiv fequiv interp_type interp_expr fcompose ftensor liftc coin xor' units type_rect delete].
+    cbv [equiv fequiv interp_type interp_expr fcompose ftensor liftc units type_rect type_rec interp_fconst interp_box interp_box_const ccompose ctensor].
     intros _.
     repeat (setoid_rewrite Bind_Ret_l || setoid_rewrite <-Bind_assoc).
     cbv [Comp_eq image_relation pointwise_relation evalDist getSupport
@@ -191,69 +644,47 @@ Section ExampleCoins.
         reflexivity.
   Qed.
 
-  Fixpoint associate_type (t : type) : type :=
-    match t with
-    | tprod t1 t2 =>
-      match associate_type t1 with
-      | tunit => associate_type t2
-      | t1' => match associate_type t2 with
-               | tunit => t1'
-               | tprod t2a t2b => tprod (tprod t1' t2a) t2b
-               | t2' => tprod t1' t2'
-               end
-      end
-    | _ => t
-    end.
-
-  Fixpoint associate (t : type) : cfunc t (associate_type t).
-    cbv [cfunc].
-    induction t; cbn [associate_type]; eauto.
-    intros [x y].
-    destruct (associate_type t1);
-      [eauto |
-       destruct (associate_type t2);
-       [apply IHt1; eauto |
-        split; [apply IHt1 | apply IHt2]; eauto |
-        split; [apply IHt1 | apply IHt2]; eauto |
-        split; [split|]; [apply IHt1; eauto|..];
-        edestruct IHt2; eauto] ..].
-  Defined.
-
-  Definition unassociate (t : type) : cfunc (associate_type t) t.
-    cbv [cfunc].
-    induction t; cbn [associate_type interp_type]; eauto.
-    intros x.
-    destruct (associate_type t1); cbn [interp_type] in *;
-      [eauto using pair, tt |
-       destruct (associate_type t2); cbn [interp_type] in *;
-       [split; [apply IHt1 | apply IHt2]; eauto using tt |
-        destruct x as [x y]; split; [apply IHt1; exact x |
-                                     apply IHt2; exact y] .. |
-        destruct x as ((x&y)&z); split; [apply IHt1; exact x |
-                                         apply IHt2; exact (y, z)] ] ..].
-  Defined.
-
   Example coins_example : expr tunit (tbool * (tbool * tbool)) :=
-    ([[units (tunit * tmap nil)]]
+    ([[units (tunit * tlist nil)]]
       @ (#coin * [[id]])
-       @ [[fadd 0]]
        @ [[copy]]
        @ (([[delete]] @ #coin) * [[id]])
-       @ [[fadd 1]]
        @ [[copy]]
        @ (([[delete]] @ #coin) * [[id]])
-       @ [[fadd 2]]
        @ [[copy]]
        @ ((([[copy]] @ ([[copy]] * [[id]]))
-             @ (let m := (madd 2 tbool (madd 1%nat tbool (madd 0%nat tbool mempty))) in
-                [[delete]] * [[find m 0]] * [[find m 2]])
+             @ (let m := (cons tbool (cons tbool (cons tbool nil))) in
+                [[delete]] * [[index m 2]] * [[index m 0]])
              @ [[associate (tunit * tbool * tbool)]]
-             @ [[xor']])
+             @ [[#bxor]])
           * [[id]])
-       @ [[fadd 3]]
        @ ([[copy]] @ ([[id]] * ([[copy]] @ ([[id]] * [[copy]]))))
-       @ (let m := (madd 3 tbool (madd 2 tbool (madd 1%nat tbool (madd 0%nat tbool mempty)))) in
-          [[find m 3]] * ([[find m 1]] * ([[find m 1]] * [[delete]])))
+       @ (let m := (cons tbool (cons tbool (cons tbool (cons tbool nil)))) in
+          [[index m 0]] * ([[index m 2]] * ([[index m 2]] * [[delete]])))
        @ [[associate (tbool * (tbool * (tbool * tunit)))]]
        @ [[unassociate (tbool * (tbool * tbool))]])%expr.
+
+  Derive coins_endpoint
+         SuchThat (equiv coins_example coins_endpoint)
+         As coins_example_rewrite.
+  Proof.
+    subst coins_endpoint.
+    cbv [coins_example].
+
+    setoid_rewrite <-compose_assoc with
+        (h :=
+           ([[associate (tbool * (tbool * (tbool * tunit)))]]
+              @
+              [[unassociate (tbool * (tbool * tbool))]])%expr).
+
+    setoid_rewrite compose_assoc with
+        (f := [[copy]]%expr).
+    setoid_rewrite interchange.
+    setoid_rewrite compose_assoc with
+        (f := [[copy]]%expr)
+        (g := ([[id]] * [[copy]])%expr).
+    setoid_rewrite interchange.
+
+    setoid_rewrite id_l.
+  Abort.
 End ExampleCoins.
